Add a few lemmas

src/circuits/dependent_test.lean
@@ -1,158 +1,158 @@
-import circuits.circuit_encoding
-import polytime.data_structures.finset
+-- import circuits.circuit_encoding
+-- import polytime.data_structures.finset
 
-namespace function
-/- Note that Lean fails to infer something like
-(infer_instance : ∀ x : α, has_uncurry (list (β x) → list (β x) → list (β x)) _ _)
-unless all the underscores are made explicit for some reason.
-(infer_instance : ∀ x : α, has_uncurry (list (β x) → list (β x) → list (β x)) (list (β x) × list (β x)) (list $ β x))
+-- namespace function
+-- /- Note that Lean fails to infer something like
+-- (infer_instance : ∀ x : α, has_uncurry (list (β x) → list (β x) → list (β x)) _ _)
+-- unless all the underscores are made explicit for some reason.
+-- (infer_instance : ∀ x : α, has_uncurry (list (β x) → list (β x) → list (β x)) (list (β x) × list (β x)) (list $ β x))
 
-This is why we make the following instances
--/
-universes u v
-variables {α : Type} {β β₁ β₂ γ δ : α → Type}
+-- This is why we make the following instances
+-- -/
+-- universes u v
+-- variables {α : Type} {β β₁ β₂ γ δ : α → Type}
 
-class has_uncurry_dep {α : Type} (β : α → Type) (β₁ β₂ : out_param (α → Type)) :=
-(uncurry : ∀ {x}, (β x) → ((β₁ x) → (β₂ x)))
+-- class has_uncurry_dep {α : Type} (β : α → Type) (β₁ β₂ : out_param (α → Type)) :=
+-- (uncurry : ∀ {x}, (β x) → ((β₁ x) → (β₂ x)))
 
-notation (name := uncurry_dep) `↾`:max x:max := has_uncurry_dep.uncurry _ x
+-- notation (name := uncurry_dep) `↾`:max x:max := has_uncurry_dep.uncurry _ x
 
-instance has_uncurry_dep_base : has_uncurry_dep (λ x, (β₁ x → β₂ x)) β₁ β₂ := ⟨λ x y, y⟩
+-- instance has_uncurry_dep_base : has_uncurry_dep (λ x, (β₁ x → β₂ x)) β₁ β₂ := ⟨λ x y, y⟩
 
-instance has_uncurry_dep_induction [has_uncurry_dep γ β₁ β₂] : has_uncurry_dep (λ x, δ x → γ x) (λ x, δ x × β₁ x) β₂ :=
-⟨λ x f p, ↾(f p.1) p.2⟩
+-- instance has_uncurry_dep_induction [has_uncurry_dep γ β₁ β₂] : has_uncurry_dep (λ x, δ x → γ x) (λ x, δ x × β₁ x) β₂ :=
+-- ⟨λ x f p, ↾(f p.1) p.2⟩
 
-end function
+-- end function
 
-open_locale complexity_class
-open function tencodable
+-- open_locale complexity_class
+-- open function tencodable
 
-namespace complexity_class
+-- namespace complexity_class
 
-variables {α : Type} {β : α → Type} {β₁ : α → Type} {β₂ : α → Type} {γ δ : Type}
-  [tencodable α] [∀ x, tencodable (β x)] [∀ x, tencodable (β₁ x)] [∀ x, tencodable (β₂ x)]
-  [tencodable γ] [tencodable δ] {C : complexity_class}
+-- variables {α : Type} {β : α → Type} {β₁ : α → Type} {β₂ : α → Type} {γ δ : Type}
+--   [tencodable α] [∀ x, tencodable (β x)] [∀ x, tencodable (β₁ x)] [∀ x, tencodable (β₂ x)]
+--   [tencodable γ] [tencodable δ] {C : complexity_class}
 
-/-- Membership of a dependent function in a complexity class;
-  Note: we only ever need *one* dependent argument for almost everything we do
+-- /-- Membership of a dependent function in a complexity class;
+--   Note: we only ever need *one* dependent argument for almost everything we do
   
-  TODO: can we unify `mem_dep` ("base case") and `mem_dep₂`?
-  Can we and should we use has_uncurry_dep so that `mem_dep₂` is automatically
-  generalized for >2 arguments?
+--   TODO: can we unify `mem_dep` ("base case") and `mem_dep₂`?
+--   Can we and should we use has_uncurry_dep so that `mem_dep₂` is automatically
+--   generalized for >2 arguments?
   
-  Should we generate composition lemmas for `mem_dep` and `mem_dep₂`? If so, what are they?  -/
-def mem_dep (f : ∀ x, β x) (C : complexity_class) : Prop :=
-∃ (f' : tree unit → tree unit), f' ∈ₑ C ∧
-  ∀ x : α, f' (encode x) = encode (f x)
+--   Should we generate composition lemmas for `mem_dep` and `mem_dep₂`? If so, what are they?  -/
+-- def mem_dep (f : ∀ x, β x) (C : complexity_class) : Prop :=
+-- ∃ (f' : tree unit → tree unit), f' ∈ₑ C ∧
+--   ∀ x : α, f' (encode x) = encode (f x)
 
-localized "infix ` ∈ₐ `:50 := complexity_class.mem_dep" in complexity_class
+-- localized "infix ` ∈ₐ `:50 := complexity_class.mem_dep" in complexity_class
 
-/-- `fintype` but "C"-constructible -/
-def mem_types (β : α → Type) [∀ x, tencodable (β x)] [∀ x, decidable_eq (β x)]
-  [∀ x, fintype (β x)] (C : complexity_class) : Prop :=
-(λ x : α, @finset.univ (β x) _) ∈ₐ C
+-- /-- `fintype` but "C"-constructible -/
+-- def mem_types (β : α → Type) [∀ x, tencodable (β x)] [∀ x, decidable_eq (β x)]
+--   [∀ x, fintype (β x)] (C : complexity_class) : Prop :=
+-- (λ x : α, @finset.univ (β x) _) ∈ₐ C
 
-def mem_dep₂ (f : ∀ x, β₁ x → β₂ x) (C : complexity_class) : Prop :=
-(λ x : sigma β₁, f x.1 x.2) ∈ₐ C
+-- def mem_dep₂ (f : ∀ x, β₁ x → β₂ x) (C : complexity_class) : Prop :=
+-- (λ x : sigma β₁, f x.1 x.2) ∈ₐ C
 
--- "t" for "two" ??
-localized "infix ` ∈ₜ `:50 := complexity_class.mem_dep₂" in complexity_class
-open_locale tree
+-- -- "t" for "two" ??
+-- localized "infix ` ∈ₜ `:50 := complexity_class.mem_dep₂" in complexity_class
+-- open_locale tree
 
-@[simp] lemma mem_dep_iff {f : α → γ} : f ∈ₐ C ↔ f ∈ₑ C :=
-by { simp_rw [mem_dep, ← prop_iff_mem], refl, }
+-- @[simp] lemma mem_dep_iff {f : α → γ} : f ∈ₐ C ↔ f ∈ₑ C :=
+-- by { simp_rw [mem_dep, ← prop_iff_mem], refl, }
 
-lemma mem_dep₂_iff {f : α → γ → δ} : f ∈ₜ C ↔ f ∈ₑ C :=
-by { dunfold mem_dep₂, rw mem_dep_iff, split; { rintro ⟨f', pf, hf⟩, refine ⟨f', pf, _⟩, rintro ⟨a, b⟩, exact hf ⟨a, b⟩, }, }
+-- lemma mem_dep₂_iff {f : α → γ → δ} : f ∈ₜ C ↔ f ∈ₑ C :=
+-- by { dunfold mem_dep₂, rw mem_dep_iff, split; { rintro ⟨f', pf, hf⟩, refine ⟨f', pf, _⟩, rintro ⟨a, b⟩, exact hf ⟨a, b⟩, }, }
 
-@[complexity] lemma mem_dep_of_mem {f : α → γ} (h : f ∈ₑ C) : f ∈ₐ C := by rwa mem_dep_iff
-@[complexity] lemma mem_dep₂_of_mem {f : α → γ → δ} (h : f ∈ₑ C) : f ∈ₜ C := by rwa mem_dep₂_iff 
+-- @[complexity] lemma mem_dep_of_mem {f : α → γ} (h : f ∈ₑ C) : f ∈ₐ C := by rwa mem_dep_iff
+-- @[complexity] lemma mem_dep₂_of_mem {f : α → γ → δ} (h : f ∈ₑ C) : f ∈ₜ C := by rwa mem_dep₂_iff 
 
-lemma mem_iff_comp_encode_dep {f : ∀ x, β x} :
-  f ∈ₐ C ↔ (λ x, encode (f x)) ∈ₑ C :=
-by { rw ← mem_dep_iff, refl, }
+-- lemma mem_iff_comp_encode_dep {f : ∀ x, β x} :
+--   f ∈ₐ C ↔ (λ x, encode (f x)) ∈ₑ C :=
+-- by { rw ← mem_dep_iff, refl, }
 
-lemma _root_.list.encode_map_encode (l : list α) :
-  encode (l.map encode) = encode l := by simp only [encode, list.map_id]
+-- lemma _root_.list.encode_map_encode (l : list α) :
+--   encode (l.map encode) = encode l := by simp only [encode, list.map_id]
 
-lemma mem_iff_comp_list_encode_dep {f : ∀ x, list (β x)} :
-  f ∈ₐ C ↔ (λ x, (f x).map encode) ∈ₑ C :=
-by { rw [mem_iff_comp_encode, mem_iff_comp_encode_dep], simp only [list.encode_map_encode], }
+-- lemma mem_iff_comp_list_encode_dep {f : ∀ x, list (β x)} :
+--   f ∈ₐ C ↔ (λ x, (f x).map encode) ∈ₑ C :=
+-- by { rw [mem_iff_comp_encode, mem_iff_comp_encode_dep], simp only [list.encode_map_encode], }
 
-end complexity_class
+-- end complexity_class
 
-/-- A function which is encoded as a table -/
-structure complexity_class.table_fun (α β : Type*) :=
-(to_fun : α → β)
+-- /-- A function which is encoded as a table -/
+-- structure complexity_class.table_fun (α β : Type*) :=
+-- (to_fun : α → β)
 
-namespace complexity_class.table_fun
-open_locale complexity_class
-variables {α β γ : Type*}
+-- namespace complexity_class.table_fun
+-- open_locale complexity_class
+-- variables {α β γ : Type*}
 
-localized "infixr ` [→] `:25 := complexity_class.table_fun" in complexity_class
+-- localized "infixr ` [→] `:25 := complexity_class.table_fun" in complexity_class
 
-instance : has_coe_to_fun (α [→] β) (λ _, α → β) := ⟨table_fun.to_fun⟩
+-- instance : has_coe_to_fun (α [→] β) (λ _, α → β) := ⟨table_fun.to_fun⟩
 
-@[ext]
-protected lemma ext : ∀ (f g : α [→] β), ⇑f = (by exact ⇑g) → f = g
-| ⟨f⟩ ⟨g⟩ rfl := rfl
+-- @[ext]
+-- protected lemma ext : ∀ (f g : α [→] β), ⇑f = (by exact ⇑g) → f = g
+-- | ⟨f⟩ ⟨g⟩ rfl := rfl
 
-@[simp] lemma to_fun_eq_coe (f : α [→] β) : f.to_fun = ⇑f := rfl
+-- @[simp] lemma to_fun_eq_coe (f : α [→] β) : f.to_fun = ⇑f := rfl
 
-@[simps]
-def equiv_fun : (α [→] β) ≃ (α → β) := ⟨λ f, ⇑f, λ f, ⟨f⟩, λ f, by ext; refl, λ f, rfl⟩
+-- @[simps]
+-- def equiv_fun : (α [→] β) ≃ (α → β) := ⟨λ f, ⇑f, λ f, ⟨f⟩, λ f, by ext; refl, λ f, rfl⟩
 
-@[simps]
-def sum (f : α [→] γ) (g : β [→] γ) : α ⊕ β [→] γ := ⟨sum.elim ⇑f ⇑g⟩
+-- @[simps]
+-- def sum (f : α [→] γ) (g : β [→] γ) : α ⊕ β [→] γ := ⟨sum.elim ⇑f ⇑g⟩
 
-@[simps]
-def map (f : α [→] β) (g : β → γ) : α [→] γ := ⟨λ x, g (f x)⟩
+-- @[simps]
+-- def map (f : α [→] β) (g : β → γ) : α [→] γ := ⟨λ x, g (f x)⟩
 
-@[simps]
-def comp (f : α [→] β) (g : γ [→] α) : γ [→] β := ⟨λ x, f (g x)⟩
+-- @[simps]
+-- def comp (f : α [→] β) (g : γ [→] α) : γ [→] β := ⟨λ x, f (g x)⟩
 
-def finmap_equiv_fun [fintype α] [decidable_eq α] :
-  {x : @finmap α (λ _, β) // ∀ k : α, k ∈ x} ≃ (α → β) :=
-{ to_fun := λ f x, @option.get _ ((↑f : finmap _).lookup x) (finmap.lookup_is_some.mpr $ f.prop x),
-  inv_fun := λ f, ⟨finmap.of_fun f, λ k, finmap.mem_iff.mpr ⟨_, finmap.of_fun_lookup k⟩⟩,
-  left_inv := λ f, by { ext : 1, apply finmap.ext_lookup, simp, },
-  right_inv := λ f, by { ext, simp, } } 
+-- def finmap_equiv_fun [fintype α] [decidable_eq α] :
+--   {x : @finmap α (λ _, β) // ∀ k : α, k ∈ x} ≃ (α → β) :=
+-- { to_fun := λ f x, @option.get _ ((↑f : finmap _).lookup x) (finmap.lookup_is_some.mpr $ f.prop x),
+--   inv_fun := λ f, ⟨finmap.of_fun f, λ k, finmap.mem_iff.mpr ⟨_, finmap.of_fun_lookup k⟩⟩,
+--   left_inv := λ f, by { ext : 1, apply finmap.ext_lookup, simp, },
+--   right_inv := λ f, by { ext, simp, } } 
 
-variables [tencodable α] [fintype α] [decidable_eq α] [tencodable β] [tencodable γ]
+-- variables [tencodable α] [fintype α] [decidable_eq α] [tencodable β] [tencodable γ]
 
-instance : tencodable (α [→] β) :=
-tencodable.of_equiv _ (equiv_fun.trans finmap_equiv_fun.symm)
+-- instance : tencodable (α [→] β) :=
+-- tencodable.of_equiv _ (equiv_fun.trans finmap_equiv_fun.symm)
 
-lemma encode_table_fun (f : α [→] β) : encode f = encode (finmap_equiv_fun.symm ⇑f) :=
-rfl
+-- lemma encode_table_fun (f : α [→] β) : encode f = encode (finmap_equiv_fun.symm ⇑f) :=
+-- rfl
 
-lemma table_fun_mk_of {γ : Type} {ψ₁ ψ₂ : γ → Type} [tencodable γ] [∀ x, tencodable (ψ₁ x)] 
-  [∀ x, fintype (ψ₁ x)] [∀ x, decidable_eq (ψ₁ x)] [∀ x, tencodable (ψ₂ x)] {f : ∀ x, (ψ₁ x → ψ₂ x)}
-  (hψ : polytime.mem_types ψ₁) (hf : f ∈ₜ PTIME) : (λ x, table_fun.mk (f x) : ∀ x, ψ₁ x [→] ψ₂ x) ∈ₐ PTIME := 
-sorry
+-- lemma table_fun_mk_of {γ : Type} {ψ₁ ψ₂ : γ → Type} [tencodable γ] [∀ x, tencodable (ψ₁ x)] 
+--   [∀ x, fintype (ψ₁ x)] [∀ x, decidable_eq (ψ₁ x)] [∀ x, tencodable (ψ₂ x)] {f : ∀ x, (ψ₁ x → ψ₂ x)}
+--   (hψ : polytime.mem_types ψ₁) (hf : f ∈ₜ PTIME) : (λ x, table_fun.mk (f x) : ∀ x, ψ₁ x [→] ψ₂ x) ∈ₐ PTIME := 
+-- sorry
 
-end complexity_class.table_fun
+-- end complexity_class.table_fun
 
-namespace polytime
-open_locale complexity_class
-open_locale tree
-open complexity_class
+-- namespace polytime
+-- open_locale complexity_class
+-- open_locale tree
+-- open complexity_class
 
-variables {α : Type} {β : α → Type} {β₁ : α → Type} {β₂ : α → Type} {γ δ : Type}
-  [tencodable α] [∀ x, tencodable (β x)] [∀ x, tencodable (β₁ x)] [∀ x, tencodable (β₂ x)]
-  [tencodable γ] [tencodable δ] {C : complexity_class}
+-- variables {α : Type} {β : α → Type} {β₁ : α → Type} {β₂ : α → Type} {γ δ : Type}
+--   [tencodable α] [∀ x, tencodable (β x)] [∀ x, tencodable (β₁ x)] [∀ x, tencodable (β₂ x)]
+--   [tencodable γ] [tencodable δ] {C : complexity_class}
 
-@[complexity] lemma list_map_dep {l : ∀ x, list (β₁ x)} {f : ∀ x, β₁ x → β₂ x} (hl : l ∈ₐ PTIME)
-  (hf : f ∈ₜ PTIME) : (λ x : α, (l x).map (f x) : ∀ x, list (β₂ x)) ∈ₐ PTIME :=
-begin
-  rcases hf with ⟨f', pf, hf⟩,
-  rw mem_iff_comp_list_encode_dep at ⊢ hl,
-  complexity using λ x, ((l x).map encode).map (λ y, f' (encode x △ y)),
-  simp at hf, dsimp [tencodable.encode_sigma] at hf, simp [function.comp, hf],
-end
+-- @[complexity] lemma list_map_dep {l : ∀ x, list (β₁ x)} {f : ∀ x, β₁ x → β₂ x} (hl : l ∈ₐ PTIME)
+--   (hf : f ∈ₜ PTIME) : (λ x : α, (l x).map (f x) : ∀ x, list (β₂ x)) ∈ₐ PTIME :=
+-- begin
+--   rcases hf with ⟨f', pf, hf⟩,
+--   rw mem_iff_comp_list_encode_dep at ⊢ hl,
+--   complexity using λ x, ((l x).map encode).map (λ y, f' (encode x △ y)),
+--   simp at hf, dsimp [tencodable.encode_sigma] at hf, simp [function.comp, hf],
+-- end
 
-@[complexity] lemma list_append_dep {l₁ l₂ : ∀ x, list (β x)} (hl₁ : l₁ ∈ₐ PTIME) (hl₂ : l₂ ∈ₐ PTIME) :
-  (λ x, (l₁ x) ++ (l₂ x)) ∈ₐ PTIME :=
-by { rw [mem_iff_comp_list_encode_dep] at *, simp only [list.map_append], complexity, }
+-- @[complexity] lemma list_append_dep {l₁ l₂ : ∀ x, list (β x)} (hl₁ : l₁ ∈ₐ PTIME) (hl₂ : l₂ ∈ₐ PTIME) :
+--   (λ x, (l₁ x) ++ (l₂ x)) ∈ₐ PTIME :=
+-- by { rw [mem_iff_comp_list_encode_dep] at *, simp only [list.map_append], complexity, }
 
-end polytime
+-- end polytime
