src/encode.lean
@@ -285,7 +285,6 @@ instance : tencodable (multiset α) :=
 (list.is_setoid α).tencodable (multiset.sort lift_le) (multiset.sort_eq _)
 
 lemma encode_multiset (x : multiset α) : encode x = encode (x.sort lift_le) := rfl
-lemma decode_multiset (x : tree unit) : decode (multiset α) x = (decode (list α) x).map quotient.mk := rfl
 
 instance [decidable_eq α] : tencodable (finset α) :=
 of_equiv {val : multiset α // val.nodup}
@@ -295,11 +294,6 @@ of_equiv {val : multiset α // val.nodup}
   right_inv := λ ⟨x, h⟩, rfl }
 
 lemma encode_finset [decidable_eq α] (x : finset α) : encode x = encode x.val := rfl
-lemma decode_finset' [decidable_eq α] (x : tree unit) : decode (finset α) x = 
-  ((decode (multiset α) x).bind $ λ y, if h : y.nodup then some (subtype.mk y h) else none).bind (λ y, some ⟨y.1, y.2⟩) := rfl
-lemma decode_finset [decidable_eq α] (x : tree unit) : decode (finset α) x = 
-  ((decode (multiset α) x).bind $ λ y, if h : y.nodup then some ⟨y, h⟩ else none) :=
-by { rw decode_finset', rw [← option.map, option.map_bind'], simp [apply_dite (option.map _)], }
 
 end finset
 
@@ -314,6 +308,9 @@ of_equiv {val : multiset (sigma β) // val.nodupkeys}
   inv_fun := λ x, ⟨x.1, x.2⟩,
   left_inv := λ ⟨x₁, x₂⟩, rfl,
   right_inv := λ ⟨x₁, x₂⟩, rfl }
+
+lemma encode_finmap [decidable_eq α] {β : α → Type*} [∀ i, tencodable (β i)] (x : finmap β) :
+  encode x = encode x.entries := rfl
 
 end finmap
 
